theories/iris/logrel/instr/typing/call_indirect.v
@@ -32,7 +32,7 @@ Section call_indirect.
     let WL := wl ++ wl' ++ wlf in
     let lmask := wlmask fe wl in
     let κ := VALTYPE (AtomR I32R) NoRefs in
-    let ψ := InstrT (τs1 ++ [CodeRefT κ (MonoFunT τs1 τs2)]) τs2 in
+    let ψ := InstrT (τs1 ++ [CodeRefT κ (InnerFunT (MonoFunT τs1 τs2))]) τs2 in
     has_instruction_type_ok F ψ L ->
     run_codegen (compile_instr mr fe (ICallIndirect ψ)) wt wl = inr ((), wt', wl', es') ->
     ⊢ have_instr_type_sem rti sr mr M F L WT WL lmask es' ψ L.
